ap/pw_ge.lean
@@ -10,9 +10,9 @@ open_locale classical
 def mk_angel_pw_ge {pw pw₁ : ℕ} (a : Angel pw)
   (h₁ : pw ≤ pw₁) : Angel pw₁ :=
 begin
-  refine ⟨λ s h, _⟩,
+  refine ⟨λ s hs h, _⟩,
   refine dite (angel_has_valid_move pw s.board) (λ h₂, _) (λ h₂, _),
-  { have v := a.f s h₂, refine ⟨v.1, v.2.1, v.2.2.1.trans h₁, v.2.2.2⟩ },
+  { have v := a.f s hs h₂, refine ⟨v.1, v.2.1, v.2.2.1.trans h₁, v.2.2.2⟩ },
   { refine ⟨_, h.some_spec⟩ },
 end
 
@@ -20,8 +20,8 @@ lemma sup_mk_angel_pw_ge {pw pw₁ : ℕ} {a : Angel pw}
   {h : pw ≤ pw₁} :
   (mk_angel_pw_ge a h).sup a :=
 begin
-  rintro b h₁, have h₂ := angel_has_valid_move_ge_of h h₁, use h₂,
-  change Valid_angel_move.m (dite _ _ _) = _, rw dif_pos h₁,
+  rintro s hs h₁, have h₂ := angel_has_valid_move_ge_of h h₁,
+  use [hs, h₂], simp_rw [mk_angel_pw_ge, dif_pos h₁],
 end
 
 lemma angel_has_valid_move_of_exi_sub {pw pw₁ : ℕ}
@@ -29,14 +29,17 @@ lemma angel_has_valid_move_of_exi_sub {pw pw₁ : ℕ}
   (h₁ : ∃ (a : Angel pw), a.sub a₁)
   (h₂ : angel_has_valid_move pw b) :
   angel_has_valid_move pw₁ b :=
-(h₁.some_spec ⟨b, []⟩ h₂).some
+(h₁.some_spec (init_state b) trivial ⟨_, h₂.some_spec⟩).some_spec.some
 
 lemma sup_angel_play_angel_move_at_eq {pw pw₁ pw₂ : ℕ}
-  {g : Game pw} {a₁ : Angel pw₁} {a₂ : Angel pw₂}
+  {g : Game pw} {a₁ : Angel pw₁} {a₂ : Angel pw₂} {hs : g.act}
   (h₁ : a₂.sup a₁)
   (h₂ : angel_has_valid_move pw₁ g.s.board) :
-  ∃ h₃, play_angel_move_at' a₂ g h₃ = play_angel_move_at' a₁ g h₂ :=
-by { obtain ⟨h₃, h₅⟩ := h₁ g.s h₂, use h₃, simp_rw [play_angel_move_at', h₅] }
+  ∃ h₃, play_angel_move_at' a₂ g hs h₃ = play_angel_move_at' a₁ g hs h₂ :=
+begin
+  obtain ⟨hs, h₃, h₅⟩ := h₁ g.s hs h₂, use h₃,
+  simp_rw play_angel_move_at', congr',
+end
 
 lemma sup_angel_play_eq {pw pw₁ n : ℕ}
   {g : Game pw} {a₁ : Angel pw₁}
@@ -57,7 +60,7 @@ begin
   rw play_move_at_act act_g₁,
   rw play_move_at_act act_g₁_a₁,
   simp_rw play_devil_move_at_set_angel,
-  let g₂ := _, change play_devil_move_at g₁ with g₂,
+  let g₂ := _, change play_devil_move_at g₁ act_g₁ with g₂,
   have hvm_pw : angel_has_valid_move pw g₂.s.board,
   { exact angel_has_valid_move_at_play_devil_move wins_at_g₁ },
   have hvm_pw₁ : angel_has_valid_move pw₁ g₂.s.board,
@@ -66,8 +69,11 @@ begin
   { exact hvm_pw },
   have hvm_pw₁' : angel_has_valid_move pw₁ (g₂.set_angel a₁).s.board,
   { exact hvm_pw₁ },
-  rw (play_angel_move_hvm hvm_pw).some_spec,
-  rw (play_angel_move_hvm hvm_pw₁').some_spec,
+  have act_g₂ : g₂.act := act_g₁,
+  have act_g₂_a₁ : (g₂.set_angel a₁).act := act_g₂,
+  rw (play_angel_move_hvm act_g₂ hvm_pw).some_spec,
+  change play_angel_move_at (g₂.set_angel a₁) = _,
+  rw (play_angel_move_hvm act_g₂_a₁ hvm_pw₁').some_spec,
   generalize_proofs,
   change (g₂.set_angel a₁).a with a₁,
   have g₁_a_eq : g₁.a = a := play_at_players_eq.1,
@@ -75,8 +81,8 @@ begin
   { convert_to g₂.a = g₁.a, { exact g₁_a_eq.symm },
     exact play_devil_move_at_players_eq.1 },
   rw g₂_a_eq,
-  have h₃ : play_angel_move_at' a₁ (g₂.set_angel a₁) hvm_pw₁ =
-    play_angel_move_at' a (g₂.set_angel a₁) hvm_pw',
+  have h₃ : play_angel_move_at' a₁ (g₂.set_angel a₁) act_g₂_a₁ hvm_pw₁ =
+    play_angel_move_at' a (g₂.set_angel a₁) act_g₂_a₁ hvm_pw',
   { exact (sup_angel_play_angel_move_at_eq h₂ _).some_spec },
   rw h₃, refl,
 end
