ap/state.lean
@@ -10,6 +10,17 @@ open_locale classical
 structure State : Type :=
 (board : Board)
 (history : list Board)
+(act : Prop)
 
-def state₀ : State := ⟨board₀, []⟩
+def init_state (b : Board) : State :=
+{ board := b,
+  history := [],
+  act := true }
+
+def state₀ : State :=
+init_state board₀
+
 instance : inhabited State := ⟨state₀⟩
+
+def State.finish (s : State) : State :=
+{s with act := false}
