ap/determinacy.lean
@@ -24,20 +24,21 @@ end
 
 -----
 
+lemma act_of_not_devil_hws {pw : ℕ} {s : State}
+  (h : ¬devil_hws_at pw s) : s.act :=
+by { contrapose! h, use default, intro a, use 0 }
+
 lemma angel_hvm_of_not_devil_hws {pw : ℕ} {s : State}
   (h : ¬devil_hws_at pw s) :
   ∀ (md : Valid_devil_move s.board),
   angel_has_valid_move pw (apply_devil_move s md.m).board :=
 begin
-  rintro md, change ¬∃ _, _ at h, push_neg at h,
-  let d := (default : Devil).set_move s md,
-  specialize h d, cases h with a h, rw not_devil_wins_at at h,
-  specialize h 1, change Game.act (Game.play_move _) at h,
-  rw init_game_play_move at h, rw play_angel_move_at at h,
-  split_ifs at h with h₁,
-  { convert h₁, symmetry, change ((default : Devil).set_move s md).f s = md,
-    exact devil_set_move_eq },
-  { cases h },
+  intro md, rw devil_hws_at at h, push_neg at h,
+  let d := (default : Devil).set_move s md, specialize h d,
+  cases h with a h, rw not_devil_wins_at at h, specialize h 1, rw play_1 at h,
+  rw Game.play_move at h, split_ifs at h with h₁, swap, { contradiction }, 
+  rw play_angel_move_at at h, split_ifs at h with h₂, swap, { cases h },
+  cases h₂ with h₂ h₃, convert h₃, change _ = dite _ _ _, rw dif_pos; refl,
 end
 
 lemma exi_moves_hws_of_not_devil_hws {pw : ℕ} {s : State}
@@ -46,26 +47,28 @@ lemma exi_moves_hws_of_not_devil_hws {pw : ℕ} {s : State}
   ∃ (ma : Valid_angel_move pw (apply_devil_move s md.m).board) (a : Angel pw),
   (init_game a d (apply_angel_move (apply_devil_move s md.m) ma.m)).angel_wins :=
 begin
+  have hs : s.act := act_of_not_devil_hws h,
   have h₁ : ¬∃ _, _ := h, push_neg at h₁,
-  simp_rw not_devil_wins_at at h₁, rintro md d₀, let md₀ := d₀.f s,
+  simp_rw not_devil_wins_at at h₁, rintro md d₀, let md₀ := d₀.f s hs,
   let d := d₀.set_move s md, let s' := apply_devil_move s md.m,
   change apply_devil_move s md.m with s',
   have h₂ : angel_has_valid_move pw s'.board,
   { apply angel_hvm_of_not_devil_hws h },
-  specialize h₁ d, cases h₁ with a h₁, let ma := a.f s' h₂, use [ma, a],
+  specialize h₁ d, cases h₁ with a h₁, let ma := a.f s' hs h₂, use [ma, a],
   have hh : d₀ = d.set_move s md₀,
   { change d₀ = (d₀.set_move s md).set_move s md₀,
     rw [devil_set_move_set_move_eq, devil_set_move_self] },
   rw hh, have h₃ : (init_game a d (apply_angel_move s' ma.m)).angel_wins,
   { convert angel_wins_at_play_move_of h₁,
-    rw init_game_play_move, change _ = dite _ _ _,
-    have h₃ : (play_devil_move_at (init_game a d s)).s = s',
+    rw init_game_play_move hs, change _ = dite _ _ _,
+    have h₃ : (play_devil_move_at (init_game a d s) hs).s = s',
     { change apply_devil_move s _ = apply_devil_move s _,
       congr, change dite _ _ _ = md, change (init_game a d s).s with s,
       rw dif_pos rfl },
-    simp_rw h₃, rw dif_pos h₂, ext; try {refl}, rw play_angel_move_at', dsimp,
-    simp_rw h₃, change (play_devil_move_at (init_game a d s)).a with a,
-    generalize_proofs h₄, convert_to _ = apply_angel_move s' (a.f s' h₂).m,
+    simp_rw h₃, rw dif_pos, swap, { split; assumption },
+    ext; try {refl}, rw play_angel_move_at', dsimp,
+    simp_rw h₃, change (play_devil_move_at (init_game a d s) hs).a with a,
+    generalize_proofs h₄, convert_to _ = apply_angel_move s' (a.f s' hs h₂).m,
     { simp_rw Game.set_state, congr; try {exact h₃}, convert_to trivial == trivial,
       { exact eq_true_intro h₄ }, { exact eq_true_intro h₂ }, refl }, refl },
   let g : Game pw := _, change g.angel_wins at h₃,
@@ -118,14 +121,16 @@ begin
   split_ifs with h₃, swap, { refl }, have h₅ : g.d = d := play_at_players_eq.2,
   simp_rw play_devil_move_at, change (g.set_devil D).s with g.s,
   change (g.set_devil D).d with D, rw h₅,
-  suffices h₆ : apply_devil_move g.s (D.f g.s).m =
-    apply_devil_move g.s (d.f g.s).m,
-  { rw h₆, rw ←play_angel_move_at_set_devil, refl },
+  suffices h₆ : apply_devil_move g.s (D.f g.s h₃).m =
+    apply_devil_move g.s (d.f g.s h₃).m,
+  { rw [h₆, ←play_angel_move_at_set_devil], refl },
   simp_rw apply_devil_move, congr' 3,
   have h₆ : ∃ (ma : Valid_angel_move pw s'.board),
     angel_played_move_at g.s s' ma,
   { exact ⟨_, angel_played_move_at_play (angel_played_move_at_apply_move rfl)⟩ },
-  change dite _ _ _ = _, split_ifs with hx, swap, { contradiction }, clear hx,
+  change (mk_devil_st_for_ma_exi_devil_st _).f _ _ = _,
+  rw mk_devil_st_for_ma_exi_devil_st, dsimp,
+  split_ifs with hx, swap, { contradiction }, clear hx,
   generalize_proofs h₇, change apply_devil_move s md.m with s' at h₇,
   have h₈ := h₇.some_spec, change d with h₂.some, congr,
   suffices h₉ : apply_angel_move (apply_devil_move s md.m) h₆.some.m = s₁,
@@ -138,13 +143,13 @@ def mk_angel_st_for_not_devil_hws (pw : ℕ) : Angel pw :=
 begin
   refine ⟨λ s' h, _⟩,
   apply dite (∃ (s : State) (md : Valid_devil_move s.board),
-    ¬devil_hws_at pw s ∧ s' = apply_devil_move s md.m); intro h₁,
+    ¬devil_hws_at pw s ∧ s' = apply_devil_move s md.m); rintro h₁ h₂,
   { refine (_ : ∃ (ma : Valid_angel_move pw s'.board),
       ¬devil_hws_at pw (apply_angel_move s' ma.m)).some,
     rcases h₁ with ⟨s, md, h₁, rfl⟩,
     use (exi_angel_move_hws_of_not_devil_hws h₁ _).some,
     generalize_proofs h₂, exact h₂.some_spec },
-  { exact ⟨_, h.some_spec⟩ },
+  { exact ⟨_, h₂.some_spec⟩ },
 end
 
 lemma not_devil_hws_at_play_of_not_devil_hws {pw n : ℕ} {g : Game pw}
@@ -156,9 +161,9 @@ begin
   rw play_at_succ', let g : Game pw := _,
   change ¬devil_hws_at pw g.s at ih,
   change ¬devil_hws_at pw g.play_move.s,
-  change g.play_move with ite _ _ _,
+  change g.play_move with dite _ _ _,
   split_ifs, swap, { exact ih },
-  let d := g.d, let s := g.s, let md := d.f s,
+  let d := g.d, let s := g.s, let md := d.f s h,
   let s' := apply_devil_move s md.m,
   have h₃ : ∃ (ma : Valid_angel_move pw s'.board),
     ¬devil_hws_at pw (apply_angel_move s' ma.m),
@@ -166,29 +171,31 @@ begin
   have ma := h₃.some, have h₄ := h₃.some_spec,
   convert h₄, change Game.s (dite _ _ _) = _,
   have h₅ : angel_has_valid_move pw s'.board := ⟨_, ma.h⟩,
-  change (play_devil_move_at g).s with s',
-  rw dif_pos h₅, change apply_angel_move _ _ = _, congr,
-  change g.a.f s' h₅ = _, let A : Angel pw := _, change g₀.a = A at h₁,
+  change (play_devil_move_at g h).s with s',
+  rw dif_pos, swap, { split; assumption },
+  change apply_angel_move _ _ = _, congr,
+  change g.a.f s' h h₅ = _, let A : Angel pw := _, change g₀.a = A at h₁,
   have h₆ : g.a = A := by { rw ←h₁, exact play_at_players_eq.1 },
-  rw h₆, let p := _, change dite p _ _ = _,
-  have h₇ : p := ⟨s, md, ih, rfl⟩, rw dif_pos h₇,
+  rw h₆, change (mk_angel_st_for_not_devil_hws pw).f _ _ _ = _,
+  rw mk_angel_st_for_not_devil_hws, dsimp, rw dif_pos, exact ⟨s, md, ih, rfl⟩,
 end
 
 lemma angel_hws_at_of {pw : ℕ} {s : State}
   (h : ¬devil_hws_at pw s) : angel_hws_at pw s :=
 begin
+  have hs : s.act := act_of_not_devil_hws h,
   let A := mk_angel_st_for_not_devil_hws pw, use A, rintro d n,
-  induction n with n ih, { triv }, rw play_at_succ',
+  induction n with n ih, { exact hs }, rw play_at_succ',
   let g : Game pw := _, change g.act at ih, change g.play_move.act,
-  let s := g.s, let md := d.f s, let s' := apply_devil_move s md.m,
-  rw play_move_at_act ih, have h₁ : play_devil_move_at g = g.set_state s',
-  { convert play_devil_move_eq, change apply_devil_move _ (d.f s).m = _,
+  let s := g.s, let md := d.f s ih, let s' := apply_devil_move s md.m,
+  rw play_move_at_act ih, have h₁ : play_devil_move_at g ih = g.set_state s',
+  { convert play_devil_move_eq, change apply_devil_move _ (d.f s ih).m = _,
     congr, symmetry, exact play_at_players_eq.2 },
   rw h₁, clear h₁, have h₁ : angel_has_valid_move pw s'.board,
   { have h₁ : ¬devil_hws_at pw s := not_devil_hws_at_play_of_not_devil_hws rfl h,
     exact ⟨_, (exi_angel_move_hws_of_not_devil_hws h₁ md).some.h⟩ },
   change Game.act (dite _ _ _), change (g.set_state s').s with s',
-  rw dif_pos h₁, exact ih,
+  rw dif_pos, swap, { split; assumption }, exact ih,
 end
 
 -----
